Finally got the 256-bit helper lemmas going through

src/crypto/aes/AES256_helpers_i.fst
@@ -107,7 +107,7 @@ let lemma_expand_key_256_0_corollary (key:aes_key_LE AES_256) : Lemma
   ()
 
 
-#reset-options "--z3rlimit 30"
+#reset-options "--z3rlimit 30 --initial_fuel 4 --max_fuel 4 --max_ifuel 0"
 // quad32 key expansion is equivalent to nat32 key expansion
 let rec lemma_expand_key_256 (key:aes_key_LE AES_256) (size:nat) : Lemma
   (requires size <= 15)
@@ -117,18 +117,68 @@ let rec lemma_expand_key_256 (key:aes_key_LE AES_256) (size:nat) : Lemma
   ))
   =
   lemma_expand_append key (4 * size) 60;
+  // assert (equal (expand_key AES_256 key (4 * size)) (slice (expand_key AES_256 key 60) 0 (4 * size)));
   if size = 0 then ()
   else
   (
     let i = size - 1 in
     lemma_expand_append key (4 * i) 60;
-    lemma_expand_key_256 key i;
+    lemma_expand_key_256 key i;  // Prove the quantifier above for i < size - 1
+    // Prove for i == size - 1
     (if i = 0 || i = 1 then (lemma_expand_key_256_0_corollary key)
      else (
-       lemma_expand_key_256_i key i;
+       lemma_expand_key_256_i key i; // ==> 
+       // round_key_256 prev0 prev1 i ~= (expand_key AES_256 key (4*i + 4)).[4*i, 4*i + 1, ... 4*i + 3]
+       //                             ~= (expand_key AES_256 key (4*i + 4)).[4*size - 4 ... 4*size - 1]
+       //                             ~= (expand_key AES_256 key  (4*size)).[4*size - 4 ... 4*size - 1]
+
+       let prev0 = expand_key_256 key (i - 2) in
+       let prev1 = expand_key_256 key (i - 1) in
+       assert (expand_key_256 key i == round_key_256 prev0 prev1 i);
+
+       let m = 4 * (i - 2) in
+       let n = 4 * i in
+       let v' = expand_key AES_256 key n in          // Current
+       let w' = expand_key AES_256 key (n + 4) in    // Next 4 words
+       let prev0' = Mkfour v'.[m + 0] v'.[m + 1] v'.[m + 2] v'.[m + 3] in  // Penultimate 4 words in Current
+       let prev1' = Mkfour v'.[m + 4] v'.[m + 5] v'.[m + 6] v'.[m + 7] in  // Ultimate 4 words in Current
+       assert (Mkfour w'.[n] w'.[n + 1] w'.[n + 2] w'.[n + 3] == round_key_256 prev0' prev1' i);
+       // ==> (expand_key AES_256 key (4 * i + 4)).[4*i ... 4*i + 3] == round_key_256 prev0' prev1' i
+       // ==> (expand_key AES_256 key (4 * size)).[4*size - 4 ... 4*size - 1] == round_key_256 prev0' prev1' i
+
+
+       // prev0' == (expand_key AES_256 key 4*i).[4 * (i-2) ... 4 * (i - 2) + 3]
+       // prev0  == expand_key_256 key (i - 2)
+       //                { induction hypothesis }
+       //        == s.[i-2]
+
+       //lemma_expand_append key (4 * (i-2)) 60;
+       //assert (prev0 == prev0');  // Fails here.  Succeeds below
+       assert (prev1 == prev1');   // OBSERVE
+       
+       // Definition of expand_key_256:
+       // expand_key_256 key i ==
+       //    round_key_256 (expand_key_256 key (i - 2)) (expand_key_256 key (i - 1)) i
+       
        let s = key_schedule_to_round_keys size (expand_key AES_256 key 60) in
-       assert (equal (expand_key AES_256 key (4 * i)) (slice (expand_key AES_256 key 60) 0 (4 * i)));
-       //admit();
+       // s = let round_keys = key_schedule_to_round_keys (size - 1) w in
+       //     let rk = Mkfour w.[4 * size - 4] w.[4 * size - 3] w.[4 * size - 2] w.[4 * size - 1] in
+       //     append round_keys (create 1 rk)
+       // s.[i] == s.[size - 1] 
+       //       ~=  Mkfour w.[4 * size - 4] w.[4 * size - 3] w.[4 * size - 2] w.[4 * size - 1]
+       
+       // Following is from: lemma_expand_append key (4 * i) 60;
+       //assert (equal (expand_key AES_256 key (4 * i)) (slice (expand_key AES_256 key 60) 0 (4 * i)));
+
+       let w = expand_key AES_256 key 60 in
+       assert (w.[4 * size - 4] == (expand_key AES_256 key (4*size)).[4 * size - 4]);
+       assert (w.[4 * size - 3] == (expand_key AES_256 key (4*size)).[4 * size - 3]);
+       assert (w.[4 * size - 2] == (expand_key AES_256 key (4*size)).[4 * size - 2]);
+       assert (w.[4 * size - 1] == (expand_key AES_256 key (4*size)).[4 * size - 1]);
+       assert (s.[i] == Mkfour w.[4 * size - 4] w.[4 * size - 3] w.[4 * size - 2] w.[4 * size - 1]);
+
+       assert (s.[i-2] == Mkfour w.[4 * (i - 1) - 4] w.[4 * (i - 1) - 3] w.[4 * (i - 1) - 2] w.[4 * (i - 1) - 1]);  // Needs extra fuel above
+       assert (prev0 == prev0');
        ()
      )
     )     
@@ -136,17 +186,17 @@ let rec lemma_expand_key_256 (key:aes_key_LE AES_256) (size:nat) : Lemma
 #reset-options
 
 // Refine round_key_256 to a SIMD computation
-let simd_round_key_256 (prev:quad32) (rcon:nat32) : quad32 =
-  let r = rot_word_LE (sub_word prev.hi3) *^ rcon in
-  let q = prev in
+let simd_round_key_256 (prev0 prev1:quad32) (rcon:nat32) (round:int) : quad32 =
+  let r = if round % 2 = 0 then rot_word_LE (sub_word prev1.hi3) *^ rcon else sub_word prev1.hi3 in
+  let q = prev0 in
   let q = q *^^ quad32_shl32 q in
   let q = q *^^ quad32_shl32 q in
   let q = q *^^ quad32_shl32 q in
   q *^^ Mkfour r r r r
 
 // SIMD version of round_key_256 is equivalent to scalar round_key_256
-let lemma_simd_round_key (prev:quad32) (rcon:nat32) : Lemma
-  (simd_round_key_256 prev rcon == round_key_256_rcon prev rcon)
+let lemma_simd_round_key (prev0 prev1:quad32) (rcon:nat32) (round:int) : Lemma
+  (simd_round_key_256 prev0 prev1 rcon round == round_key_256_rcon prev0 prev1 rcon round)
   =
-  commute_rot_word_sub_word prev.hi3;
+  commute_rot_word_sub_word prev1.hi3;
   Types_i.xor_lemmas ()
